Reorganize inner loop

template-coq/theories/clauses.v
@@ -67,6 +67,44 @@ Ltac clsets := ClausesDecide.fsetdec.
 
 Definition clauses := Clauses.t.
 
+Lemma filter_add {p x s} : Clauses.Equal (Clauses.filter p (Clauses.add x s)) (if p x then Clauses.add x (Clauses.filter p s) else Clauses.filter p s).
+Proof.
+  intros i.
+  rewrite Clauses.filter_spec.
+  destruct (eqb_spec i x); subst;
+  destruct (p x) eqn:px; rewrite !Clauses.add_spec !Clauses.filter_spec; intuition auto || congruence.
+Qed.
+
+Instance proper_fold_transpose {A} (f : Clauses.elt -> A -> A) :
+  transpose eq f ->
+  Proper (Clauses.Equal ==> eq ==> eq) (Clauses.fold f).
+Proof.
+  intros hf s s' Hss' x ? <-.
+  eapply ClausesProp.fold_equal; tc; tea.
+Qed.
+Existing Class transpose.
+
+Lemma clauses_fold_filter {A} (f : Clauses.elt -> A -> A) (p : Clauses.elt -> bool) cls acc : 
+  transpose Logic.eq f ->
+  Clauses.fold f (Clauses.filter p cls) acc = 
+  Clauses.fold (fun elt acc => if p elt then f elt acc else acc) cls acc.
+Proof.
+  intros hf.
+  symmetry. eapply ClausesProp.fold_rec_bis.
+  - intros s s' a eq. intros ->. 
+    eapply ClausesProp.fold_equal; tc. auto.
+    intros x.
+    rewrite !Clauses.filter_spec.
+    now rewrite eq.
+  - now cbn.
+  - intros.
+    rewrite H1.
+    rewrite filter_add.
+    destruct (p x) eqn:px => //.
+    rewrite ClausesProp.fold_add //.
+    rewrite Clauses.filter_spec. intuition auto.
+Qed.
+
 Module MoreLevel.
 
   Include Level.
@@ -107,11 +145,40 @@ Module MoreLevel.
     eapply transitivity; [exact H1|exact H0].
   Qed.
 
+  Lemma compare_eq {x y} : compare x y = Eq -> x = y.
+  Proof.
+    destruct (compare_spec x y) => //.
+  Qed.
 End MoreLevel.
 
 Module LevelOT := OrderedType_from_Alt MoreLevel.
 Module LevelMap := FMapAVL.Make LevelOT.
 Module LevelMapFact := FMapFacts.WProperties LevelMap.
+
+Definition strict_subset (s s' : LevelSet.t) :=
+  LevelSet.Subset s s' /\ ~ LevelSet.Equal s s'.
+
+Lemma strict_subset_incl (x y z : LevelSet.t) : LevelSet.Subset x y -> strict_subset y z -> strict_subset x z.
+Proof.
+  intros hs []. split => //. lsets.
+  intros heq. apply H0. lsets.
+Qed.
+
+Lemma strict_subset_cardinal s s' : strict_subset s s' -> LevelSet.cardinal s < LevelSet.cardinal s'.
+Proof.
+  intros [].
+  assert (LevelSet.cardinal s <> LevelSet.cardinal s').
+  { intros heq. apply H0. 
+    intros x. split; intros. now apply H.
+    destruct (LevelSet.mem x s) eqn:hin.
+    eapply LevelSet.mem_spec in hin.
+    auto. eapply LevelSetProp.FM.not_mem_iff in hin.
+    exfalso.
+    eapply LevelSetProp.subset_cardinal_lt in hin; tea.
+    lia. }
+  enough (LevelSet.cardinal s <= LevelSet.cardinal s') by lia.
+  now eapply LevelSetProp.subset_cardinal.
+Qed.
 
 Record model := {
   model_values :> LevelMap.t nat
@@ -167,25 +234,6 @@ Next Obligation.
   destruct l. cbn in *. congruence.    
 Qed.
 
-
-Definition strict_subset (s s' : LevelSet.t) :=
-  LevelSet.Subset s s' /\ ~ LevelSet.Equal s s'.
-
-Lemma strict_subset_cardinal s s' : strict_subset s s' -> LevelSet.cardinal s < LevelSet.cardinal s'.
-Proof.
-  intros [].
-  assert (LevelSet.cardinal s <> LevelSet.cardinal s').
-  { intros heq. apply H0. 
-    intros x. split; intros. now apply H.
-    destruct (LevelSet.mem x s) eqn:hin.
-    eapply LevelSet.mem_spec in hin.
-    auto. eapply LevelSetProp.FM.not_mem_iff in hin.
-    exfalso.
-    eapply LevelSetProp.subset_cardinal_lt in hin; tea.
-    lia. }
-  enough (LevelSet.cardinal s <= LevelSet.cardinal s') by lia.
-  now eapply LevelSetProp.subset_cardinal.
-Qed.
 
 Definition min_atom_value (m : model) (atom : LevelExpr.t) :=
   let '(l, k) := atom in
@@ -243,15 +291,15 @@ Definition update_value (wm : LevelSet.t × model) (cl : clause) : update_result
       (* The conclusion doesn't hold, we need to set it higher *)
       DoesntHold (LevelSet.add l w, update_model m l (k + Z.to_nat k0)).
 
+Definition check_clause_model cl '(modified, wm) := 
+  match update_value wm cl with 
+  | VacuouslyTrue => (modified, wm)
+  | DoesntHold wm' => (true, wm')
+  | Holds => (modified, wm)
+  end.
+
 Definition check_model_aux (cls : clauses) (wm : LevelSet.t × model) : bool × (LevelSet.t × model) :=
-  Clauses.fold
-    (fun cl '(modified, wm) => 
-      match update_value wm cl with 
-      | VacuouslyTrue => (modified, wm)
-      | DoesntHold wm' => (true, wm')
-      | Holds => (modified, wm)
-      end)
-    cls (false, wm).
+  Clauses.fold check_clause_model cls (false, wm).
 
 (* If check_model = None then we have a model of all clauses, 
   othewise, we return Some (W', m') where W ⊂ W' and the model has
@@ -264,7 +312,7 @@ Lemma check_model_aux_subset {cls w v} :
   forall b w' v', check_model_aux cls (w, v) = (b, (w', v')) -> LevelSet.Subset w w'.
 Proof.
   intros w' v'.
-  unfold check_model, check_model_aux. revert w' v'.
+  unfold check_model, check_model_aux, check_clause_model. revert w' v'.
   eapply ClausesProp.fold_rec => //.
   { intros. noconf H0. reflexivity. }
   intros x a s' s'' hin nin hadd IH.
@@ -372,8 +420,8 @@ Definition levelexpr_value : LevelExprSet.elt -> nat := snd.
 Coercion levelexpr_value : LevelExprSet.elt >-> nat.
 
 Definition v_minus_w_bound (V W : LevelSet.t) (m : model) := 
-  LevelMap.fold (fun w v acc => 
-    if LevelSet.mem w (LevelSet.diff V W) then Nat.max v acc else acc) m 0.
+  LevelMap.fold (fun w v acc => Nat.max v acc) 
+    (LevelMapFact.filter (fun l _ => LevelSet.mem l (LevelSet.diff V W)) m) 0.
   
 Definition premise_min (l : nonEmptyLevelExprSet) : nat :=
   LevelExprSet.fold (fun atom min => Nat.min atom min) l 0.
@@ -384,15 +432,7 @@ Definition gain (cl : clause) : Z :=
 Definition max_gain (cls : clauses) := 
   Clauses.fold (fun cl acc => Nat.max (Z.to_nat (gain cl)) acc) cls 0.
 
-(** The termination proof relies on the correctness of check_model: 
-  it does strictly increase a value but not above [max_gain cls].
-*)
 
-Lemma check_model_spec cls w m : 
-  forall w' m', check_model cls (w, m) = Some (w', m') -> 
-  w ⊂_lset w' /\ w' ⊂_lset (LevelSet.union w (clauses_conclusions cls)) /\
-  exists l, LevelSet.In l w' /\ level_value m l < level_value m' l <= max_gain cls.
-Proof. Admitted.
 (*  
   eapply (ClausesProp.fold_rel (R := fun x y => forall (w' : LevelSet.t) (m : model), x = Some (w', m) -> LevelSet.Subset w' (LevelSet.union w y))) => //.
   intros x a s' hin IH w' m'.
@@ -411,81 +451,100 @@ Proof. Admitted.
     intros [= <- <-]. lsets.
 Qed. *)
 
-Inductive result (V : LevelSet.t) :=
+Definition model_same_domain (m m' : model) := 
+  forall l, LevelMap.In l m <-> LevelMap.In l m'.
+
+#[local] Instance model_same_domain_refl : Reflexive model_same_domain.
+Proof. intros m l. reflexivity. Qed.
+
+#[local] Instance model_same_domain_trans : Transitive model_same_domain.
+Proof. intros m m' m'' h h' l. rewrite (h l). apply h'. Qed.
+
+Definition model_le (m m' : model) := 
+  forall l k, LevelMap.MapsTo l k m -> 
+  exists k', LevelMap.MapsTo l k' m' /\ k <= k'.
+    
+Infix "⩽" := model_le (at level 70). (* \leqslant *)
+
+Definition model_map_outside V (m m' : model) :=
+  forall l, ~ LevelSet.In l V -> 
+    forall k, LevelMap.MapsTo l k m <-> LevelMap.MapsTo l k m'.
+
+#[local] Instance model_map_outside_refl V : Reflexive (model_map_outside V).
+Proof. intros m l. reflexivity. Qed.
+
+#[local] Instance model_map_outside_trans V : Transitive (model_map_outside V).
+Proof.
+  intros m m' m'' h h' l hnin k.
+  rewrite (h l hnin k). now apply h'.
+Qed.
+
+(** The termination proof relies on the correctness of check_model: 
+  it does strictly increase a value but not above [max_gain cls].
+*)
+
+Lemma check_model_spec cls w m : 
+  forall w' m', check_model cls (w, m) = Some (w', m') -> 
+  [/\ w ⊂_lset w',
+      w' ⊂_lset (LevelSet.union w (clauses_conclusions cls)),
+      exists l, LevelSet.In l w' /\ level_value m l < level_value m' l <= max_gain cls,
+      model_same_domain m m' &
+      model_map_outside w' m m'].
+Proof. Admitted.
+
+Record valid_model (V : LevelSet.t) (m : model) (cls : clauses) :=
+  { model_model : model;
+    model_clauses_conclusions : clauses_conclusions cls ⊂_lset V;
+    model_ok : check_model cls (LevelSet.empty, model_model) = None;
+    model_above : m ⩽ model_model;
+    model_domains : model_same_domain m model_model;
+    model_outside : model_map_outside V m model_model
+ }.
+Arguments model_model {V m cls}.
+Arguments model_clauses_conclusions {V m cls}.
+Arguments model_ok {V m cls}.
+Arguments model_above {V m cls}.
+Arguments model_domains {V m cls}.
+Arguments model_outside {V m cls}.
+
+Inductive result (V : LevelSet.t) (cls : clauses) (m : model) :=
   | Loop
-  | Model (w : LevelSet.t) (m : model) (prf : LevelSet.subset w V).
-    (* (ism : check_model cls (w, m) = None). *)
-Arguments Loop {V}.
-Arguments Model {V}.
+  | Model (w : LevelSet.t) (m : valid_model V m cls) (prf : LevelSet.subset w V).
+Arguments Loop {V cls m}.
+Arguments Model {V cls m}.
 Arguments exist {A P}.  
 Definition inspect {A} (x : A) : { y : A | x = y } := exist x eq_refl.
 Arguments lexprod {A B}.
 
-Definition option_of_result {V} (r : result V) : option model :=
+Definition option_of_result {V m cls} (r : result V m cls) : option model :=
   match r with
   | Loop => None
-  | Model w m sub => Some m
+  | Model w m sub => Some m.(model_model)
   end. 
 
-Lemma filter_add {p x s} : Clauses.Equal (Clauses.filter p (Clauses.add x s)) (if p x then Clauses.add x (Clauses.filter p s) else Clauses.filter p s).
-Proof.
-  intros i.
-  rewrite Clauses.filter_spec.
-  destruct (eqb_spec i x); subst;
-  destruct (p x) eqn:px; rewrite !Clauses.add_spec !Clauses.filter_spec; intuition auto || congruence.
-Qed.
-
-Instance proper_fold_transpose {A} (f : Clauses.elt -> A -> A) :
-  transpose eq f ->
-  Proper (Clauses.Equal ==> eq ==> eq) (Clauses.fold f).
-Proof.
-  intros hf s s' Hss' x ? <-.
-  eapply ClausesProp.fold_equal; tc; tea.
-Qed.
-Existing Class transpose.
-
-Lemma clauses_fold_filter {A} (f : Clauses.elt -> A -> A) (p : Clauses.elt -> bool) cls acc : 
-  transpose Logic.eq f ->
-  Clauses.fold f (Clauses.filter p cls) acc = 
-  Clauses.fold (fun elt acc => if p elt then f elt acc else acc) cls acc.
-Proof.
-  intros hf.
-  symmetry. eapply ClausesProp.fold_rec_bis.
-  - intros s s' a eq. intros ->. 
-    eapply ClausesProp.fold_equal; tc. auto.
-    intros x.
-    rewrite !Clauses.filter_spec.
-    now rewrite eq.
-  - now cbn.
-  - intros.
-    rewrite H1.
-    rewrite filter_add.
-    destruct (p x) eqn:px => //.
-    rewrite ClausesProp.fold_add //.
-    rewrite Clauses.filter_spec. intuition auto.
-Qed.
-
-Lemma strict_subset_incl (x y z : LevelSet.t) : LevelSet.Subset x y -> strict_subset y z -> strict_subset x z.
-Proof.
-  intros hs []. split => //. lsets.
-  intros heq. apply H0. lsets.
-Qed.
-
-Definition lexprod_rel := lexprod lt lt.
+(* Definition lexprod_rel := lexprod lt lt.
 
 #[local] Instance lexprod_rel_wf : WellFounded lexprod_rel.
 Proof.
   eapply (Acc_intro_generator 1000). unfold lexprod_rel. eapply wf_lexprod, lt_wf. eapply lt_wf.
 Defined.
 
-Opaque lexprod_rel_wf.
+Opaque lexprod_rel_wf. *)
  
-Equations? result_inclusion {V V'} (r : result V) (prf : LevelSet.Subset V V') : result V' :=
+#[tactic="idtac"]
+Equations? result_inclusion {V m cls V'} (r : result V cls m) (prf : LevelSet.Subset V V') : result V' cls m :=
   result_inclusion Loop _ := Loop;
-  result_inclusion (Model w m sub) sub' := Model w m _.
+  result_inclusion (Model w m' sub) sub' := 
+    Model w {| model_model := m'.(model_model) |} _.
 Proof.
-  eapply LevelSet.subset_spec. eapply LevelSet.subset_spec in sub.
-  now transitivity V.
+  - transitivity V => //. now eapply m'.(model_clauses_conclusions).
+  - apply m'.
+  - apply m'.
+  - apply m'.
+  - intros x hin. apply m'. intros hv. apply LevelSet.subset_spec in sub.
+    apply sub' in hv. now apply hin.
+  - eapply LevelSet.subset_spec. eapply LevelSet.subset_spec in sub.
+    now transitivity V.
 Qed.
 
 
@@ -514,12 +573,13 @@ Proof.
 Qed. *)
 
 
-Lemma clauses_conclusions_diff a cls s : 
-  LevelSet.In a (clauses_conclusions (Clauses.diff cls (clauses_with_concl cls s))) -> 
-  LevelSet.In a (clauses_conclusions cls) /\ ~ LevelSet.In a s.
+Lemma clauses_conclusions_diff cls s : 
+  clauses_conclusions (Clauses.diff cls (clauses_with_concl cls s)) ⊂_lset
+  LevelSet.diff (clauses_conclusions cls) s.
 Proof.
-  rewrite !clauses_conclusions_spec.
-  firstorder eauto. exists x; split => //.
+  intros a. rewrite LevelSet.diff_spec !clauses_conclusions_spec.
+  firstorder eauto.
+  exists x; split => //.
   now rewrite Clauses.diff_spec in H.
   intros ha.
   rewrite Clauses.diff_spec in H; destruct H as [].
@@ -608,77 +668,571 @@ Proof.
   now rewrite InA_In_eq.
 Qed.
 
+Lemma clauses_empty_eq {s} : Clauses.Empty s -> Clauses.Equal s Clauses.empty.
+Proof. clsets. Qed.
+
+Lemma update_value_valid {W m cl} : 
+  match update_value (W, m) cl with
+  | VacuouslyTrue | Holds => valid_clause m cl
+  | DoesntHold _ => ~~ valid_clause m cl
+  end.
+Proof.
+  unfold update_value, valid_clause.
+  destruct Z.ltb => //.
+  destruct cl as [prem [l k]]; cbn.
+  destruct Nat.leb => //.
+Qed.
+
+Lemma valid_update_value {W m cl} : 
+  valid_clause m cl -> 
+  match update_value (W, m) cl with
+  | VacuouslyTrue | Holds => true
+  | DoesntHold _ => false
+  end.
+Proof.
+  unfold update_value, valid_clause.
+  destruct Z.ltb => //.
+  destruct cl as [prem [l k]]; cbn.
+  destruct Nat.leb => //.
+Qed.
+
+Lemma check_model_aux_false {cls acc acc'} : check_model_aux cls acc = (false, acc') -> acc = acc'.
+Proof.
+  unfold check_model_aux, check_clause_model.
+  eapply ClausesProp.fold_rec.
+  - intros s emp [=] => //.
+  - intros cl [modified [w' m']] cls' cls'' incl nincls' incls''.
+    intros IH.
+    destruct update_value eqn:upd => //.
+Qed.
+
+(* Lemma check_model_aux_true {cls acc acc'} : check_model_aux cls acc = (true, acc') -> acc = acc'.
+Proof.
+  unfold check_model_aux.
+  eapply ClausesProp.fold_rec.
+  - intros s emp [=] => //.
+  - intros cl [modified [w' m']] cls' cls'' incl nincls' incls''.
+    intros IH.
+    destruct update_value eqn:upd => //.
+Qed. *)
+
+Lemma check_model_aux_model {cls acc} : 
+  check_model_aux cls acc = (false, acc) <-> is_model cls acc.2.
+Proof.
+  unfold check_model_aux, check_clause_model.
+  unfold is_model.
+  unfold is_true; rewrite -ClausesFact.for_all_iff.
+  eapply ClausesProp.fold_rec.
+  - intros s emp.
+    split => //.
+    intros [=] x hx. clsets.
+  - intros cl [modified [w' m']] cls' cls'' incl nincls' incls''.
+    intros IH.
+    split.
+    * move: (@update_value_valid w' m' cl).
+      destruct update_value eqn:upd => //; intros vcl [= -> <-] ;
+        destruct IH as [IH _]; specialize (IH eq_refl).
+      intros x hx; apply incls'' in hx as []; subst. exact vcl. now apply IH.
+      intros x hx; apply incls'' in hx as []; subst. exact vcl. now apply IH.
+    * intros hf.
+      assert (valid_clause acc.2 cl).
+      { apply hf. apply incls''. intuition auto. }
+      destruct IH as [_ IH]. forward IH.
+      { intros x hx. apply hf. apply incls''. now right. }
+      noconf IH.
+      move: (@valid_update_value w' m' cl H).
+      destruct update_value eqn:upd => //.
+Qed.
+
+Lemma clauses_for_all_neg {p s}: 
+  ~~ Clauses.for_all p s <-> ~ Clauses.For_all p s.
+Proof.
+  intuition auto.
+  rewrite ClausesFact.for_all_iff in H0. red in H. now rewrite H0 in H.
+  revert H. apply contra_notN.
+  rewrite ClausesFact.for_all_iff //.
+Qed.
+
+Lemma clauses_for_all_exists {p s}: 
+  ~~ Clauses.for_all p s <-> Clauses.exists_ (fun x => ~~ p x) s.
+Proof.
+  rewrite ClausesFact.for_all_b ClausesFact.exists_b.
+  induction (Clauses.elements s).
+  - cbn; auto. reflexivity.
+  - cbn. rewrite negb_and. intuition auto.
+    move/orP: H1 => [->|] //. move/H. intros ->. now rewrite orb_true_r.
+    move/orP: H1 => [->|] //. move/H0. intros ->. now rewrite orb_true_r.
+Qed.
+#[local] Instance model_le_refl : Reflexive model_le.
+Proof. intros x l k map. exists k; split => //. Qed.
+
+#[local] Instance model_le_trans : Transitive model_le.
+Proof. intros m m' m'' mm' m'm'' l k map.
+  apply mm' in map as [k' [map ?]].
+  apply m'm'' in map as [k'' [map ?]]. exists k''. split => //. lia.
+Qed.
+
+Lemma update_model_monotone m l k : level_value m l <= k -> m ⩽ update_model m l k.
+Proof.
+  intros hl.
+  intros l' k' maps. 
+  unfold update_model. cbn.
+  destruct (eqb_spec l l').
+  - exists k. move: hl. subst l'.
+    unfold level_value.
+    rewrite (LevelMap.find_1 maps).
+    intros hle. 
+    split => //. eapply LevelMap.add_1. eapply LevelMap.E.eq_refl.
+  - exists k'. split => //. apply LevelMap.add_2 => //.
+    intros he. destruct (MoreLevel.compare_spec l l'); congruence.
+Qed.
+
+Lemma check_clause_model_inv {cl modified w m b wm'} : 
+  check_clause_model cl (modified, (w, m)) = (b, wm') ->
+  m ⩽ wm'.2.
+Proof.
+  unfold check_clause_model.
+  destruct (update_value (w, m) cl) eqn:upd.
+  * now intros [= <- <-].
+  * now intros [= <- <-].
+  * intros [= <- <-].
+    move: upd.
+    unfold update_value.
+    case: Z.ltb_spec => //.
+    destruct cl as [prem [l k]] => /=.
+    intros hprem.
+    case: Nat.leb_spec => // hlt.
+    intros [= <-]. cbn.
+    eapply update_model_monotone. lia.  
+Qed.
+  
+Lemma check_clause_model_intact {cl modified w m wm'} : 
+  check_clause_model cl (modified, (w, m)) = (false, wm') -> valid_clause m cl /\ wm' = (w, m).
+Proof.
+  unfold check_clause_model.
+  move: (@update_value_valid w m cl).
+  destruct (update_value (w, m) cl) eqn:upd.
+  * intros valid [= -> <-]. split => //.
+  * intros valid [= -> <-]. split => //.
+  * intros _ [=].
+Qed.
+
+Lemma check_clause_model_modify {cl w m wm'} : 
+  check_clause_model cl (false, (w, m)) = (true, wm') -> ~~ valid_clause m cl.
+Proof.
+  unfold check_clause_model.
+  destruct (update_value (w, m) cl) eqn:upd.
+  * now intros [= <- <-].
+  * now intros [= <- <-].
+  * intros [= <-].
+    move: upd.
+    unfold update_value, valid_clause.
+    case: Z.ltb_spec => //.
+    destruct cl as [prem [l k]] => /=.
+    intros hprem.
+    case: Nat.leb_spec => // hlt.
+Qed.
+
+Lemma check_model_aux_model_le {cls acc acc' b} : 
+  check_model_aux cls acc = (b, acc') -> acc.2 ⩽ acc'.2.
+Proof.
+  unfold check_model_aux.
+  revert b acc'.
+  eapply ClausesProp.fold_rec.
+  - intros s emp b acc'. intros [=]. subst. reflexivity. 
+  - intros cl [modified [w' m']] cls' cls'' incl nincls' incls''.
+    intros IH b acc'.
+    move/check_clause_model_inv.
+    specialize (IH _ _ eq_refl). cbn in IH. now intros; transitivity m'.
+Qed.
+
+Lemma check_model_aux_not_model {cls acc acc'} : 
+  check_model_aux cls acc = (true, acc') -> ~~ is_model cls acc.2.
+Proof.
+  unfold check_model_aux.
+  unfold is_model. 
+  rewrite clauses_for_all_exists /is_true ClausesFact.exists_b.
+  rewrite Clauses.fold_spec.
+  revert acc acc'. induction (Clauses.elements cls); intros acc acc'.
+  - cbn. intros [=].
+  - cbn -[check_clause_model].
+    destruct (check_clause_model a) eqn:cl.
+    destruct acc as [w m].
+    pose proof (check_clause_model_inv cl) as accle.
+    destruct b.
+    * intros _. apply/orP. left. cbn.
+      now eapply check_clause_model_modify.
+    * intros hl. specialize (IHl _ _ hl).
+      cbn. apply/orP. right.
+      apply check_clause_model_intact in cl as []. subst p. exact IHl.
+Qed.
+
+Lemma check_model_is_model {W cls m} : check_model cls (W, m) = None <-> is_model cls m.
+Proof.
+  unfold check_model, is_model.
+  destruct check_model_aux eqn:caux.
+  destruct b => //. intuition auto. congruence.
+  { eapply check_model_aux_not_model in caux.
+    rewrite /is_model /= // in caux. now rewrite H in caux. }
+  intuition auto.
+  pose proof (check_model_aux_false caux). subst p.
+  now rewrite check_model_aux_model in caux.
+Qed.
+
+Lemma check_model_update {W cls m wm'} : check_model cls (W, m) = Some wm' -> ~~ is_model cls m /\ m ⩽ wm'.2.
+Proof.
+  unfold check_model, is_model.
+  destruct check_model_aux eqn:caux.
+  destruct b => //. intros [= <-]. intuition auto. 
+  now eapply check_model_aux_not_model in caux.
+  now eapply check_model_aux_model_le in caux.
+Qed.
+
 Infix "↓" := clauses_with_concl (at level 70). (* \downarrow *)
 Infix "⇂" := restrict_clauses (at level 70). (* \downharpoonright *)
+
+Lemma is_model_union {cls cls' m} : 
+  is_model cls m -> is_model cls' m -> is_model (Clauses.union cls cls') m.
+Proof.
+  rewrite /is_model. rewrite /is_true -!ClausesFact.for_all_iff.
+  now move=> ism ism' x /Clauses.union_spec [].
+Qed.
+
+#[local] Instance Clauses_For_All_proper : Proper (eq ==> Clauses.Equal ==> iff) Clauses.For_all.
+Proof.
+  intros x y -> cl cl' eqcl.
+  unfold Clauses.For_all. now setoid_rewrite eqcl.
+Qed.
+
+#[local] Instance Clauses_for_all_proper : Proper (eq ==> Clauses.Equal ==> eq) Clauses.for_all.
+Proof.
+  intros x y -> cl cl' eqcl.
+  apply iff_is_true_eq_bool.
+  rewrite /is_true -!ClausesFact.for_all_iff. now rewrite eqcl.
+Qed.
+
+#[local] Instance is_model_proper : Proper (Clauses.Equal ==> eq ==> eq) is_model.
+Proof.
+  intros cl cl' eqcl x y ->. unfold is_model. now rewrite eqcl.
+Qed.
+
+Definition extends_model {W cls m m'} : 
+  m' ⩽ m ->
+  model_same_domain m' m ->
+  model_map_outside W m' m ->
+  result W cls m -> result W cls m'.
+Proof.
+  intros leq ldom lout []. exact Loop.
+  econstructor 2; tea.
+  destruct m0. econstructor; tea.
+  - now transitivity m.
+  - now transitivity m.
+  - now transitivity m.
+Qed.
+
+Lemma model_le_values (m m' : model) x : m ⩽ m' -> level_value m x <= level_value m' x.
+Proof.
+  intros lem. specialize (lem x).
+  unfold level_value.
+  destruct LevelMap.find eqn:hl => //. 2:lia.
+  apply LevelMap.find_2 in hl. specialize (lem _ hl) as [k' [mapsto leq]].
+  now rewrite (LevelMap.find_1 mapsto).
+Qed.
+
+Lemma level_value_MapsTo {k e} {m : model} : 
+  LevelMap.MapsTo k e m -> level_value m k = e.
+Proof.
+  unfold level_value.
+  move=> mapto; rewrite (LevelMap.find_1 mapto) //.
+Qed.
+
+Lemma model_map_outside_weaken {W W'} {m m' : model} : 
+  model_map_outside W m m' ->
+  W ⊂_lset W' ->
+  model_map_outside W' m m'.
+Proof.
+  intros hm sub x hin k.
+  apply hm. intros hin'. apply sub in hin'. now apply hin.
+Qed.
+
+Infix "⊂_clset" := Clauses.Subset (at level 70).
+
+Lemma max_gain_in cl cls : 
+  Clauses.In cl cls ->
+  Z.to_nat (gain cl) <= max_gain cls.
+Proof.
+  intros hin.
+  unfold max_gain. revert cl hin.
+  eapply ClausesProp.fold_rec.
+  - intros s' ise hin. firstorder eauto.
+  - intros x a s' s'' xs nxs' hadd IH cl' hin'.
+    eapply hadd in hin' as [].
+    * subst x. lia.
+    * specialize (IH _ H). lia.
+Qed.
+
+Definition max_gain_subset (cls cls' : Clauses.t) : 
+  cls ⊂_clset cls' ->
+  max_gain cls <= max_gain cls'.
+Proof.
+  unfold max_gain at 1.
+  revert cls'.
+  eapply ClausesProp.fold_rec.
+  - intros s' ise sub. lia.
+  - intros x a s' s'' xs nxs' hadd IH cls'' hs.
+    specialize (IH cls''). forward IH. transitivity s'' => //. 
+    intros ??. now apply hadd.
+    assert (incls'' : Clauses.In x cls'').
+    { now apply hs, hadd. }
+    apply max_gain_in in incls''. lia.
+Qed.
 
 Section InnerLoop.
   Context (V : LevelSet.t) 
     (loop : forall (V' : LevelSet.t) (cls : clauses) (m : model) (p : clauses_conclusions cls ⊂_lset V'),
-    LevelSet.cardinal V' < LevelSet.cardinal V -> result V'). 
+    LevelSet.cardinal V' < LevelSet.cardinal V -> result V' cls m). 
   
   Definition measure (W : LevelSet.t) (cls : clauses) (m : model) : nat := 
     let bound := v_minus_w_bound V W m in
+    let cls := (Clauses.diff (cls ↓ W) (cls ⇂ W)) in
     let maxgain := max_gain cls in 
     LevelSet.fold (fun w acc => 
         Nat.add acc (bound + maxgain - level_value m w)) W 0.
-  Notation cls_diff cls W := (Clauses.diff (cls ↓ W) (cls ⇂ W)).
+  Notation cls_diff cls W := (Clauses.diff (cls ↓ W) (cls ⇂ W)) (only parsing).
+  
+(*
+  Equations? extend_model {W cls} (m : valid_model W (cls ⇂ W))
+    (r : result W (Clauses.diff (cls ↓ W) (cls ⇂ W)))
+    : result W (cls ↓ W) :=
+    extend_model _ Loop := Loop;
+    extend_model m (Model w m' sub) := 
+      Model w {| model_model := m'.(model_model) |} _.
+  Proof.
+    - apply LevelSet.subset_spec in sub. now apply clauses_conclusions_clauses_with_concl in H. 
+    - eapply sub. now eapply m.(model_clauses_conclusions).
+    - apply m.
+    - eapply LevelSet.subset_spec. eapply LevelSet.subset_spec in sub.
+      now transitivity V.
+  Qed.
+  *)
+
+  Lemma v_minus_w_bound_irrel {W} m m' : 
+    model_map_outside W m m' ->
+    v_minus_w_bound V W m = v_minus_w_bound V W m'.
+  Proof.
+    unfold v_minus_w_bound.
+    intros out. eapply LevelMapFact.fold_Equal. tc. cbn.
+    { intros x y eq. cbn. solve_proper. }
+    { intros x y. cbn. intros e e' a neq. lia. }
+    apply LevelMapFact.F.Equal_mapsto_iff.
+    intros k e. rewrite -> LevelMapFact.filter_iff.
+    2:{ intros x y eq. eapply MoreLevel.compare_eq in eq. subst y. solve_proper. }
+    rewrite -> LevelMapFact.filter_iff.
+    2:{ move=> x y /MoreLevel.compare_eq ->. solve_proper. }
+    rewrite LevelSet.mem_spec LevelSet.diff_spec.
+    intuition auto.
+    - now apply out.
+    - now apply out.
+  Qed.
+  
+  Definition min_value (m : model) (atom : LevelExpr.t) :=
+    let '(l, k) := atom in
+    (Z.of_nat (level_value m l))%Z.
+  
+  Definition min_premise_value (m : model) (l : nonEmptyLevelExprSet) : Z :=
+    LevelExprSet.fold (fun atom min => Z.min (min_value m atom) min) l 
+     (min_value m (choose l)).
+
+  Definition non_W_atoms W (l : nonEmptyLevelExprSet) := 
+    LevelExprSet.filter (fun '(l, k) => ~~ LevelSet.mem l W) l.
+
+  Lemma measure_model W cls m :
+    clauses_conclusions cls ⊂_lset W ->
+    let clsdiff := cls_diff cls W in
+    measure W cls m = 0 -> is_model clsdiff m.
+  Proof using.
+    clear loop. 
+    unfold measure, is_model.
+    set (clsdiff := Clauses.diff _ _).
+    intros clw hm.
+    assert (LevelSet.For_all (fun w => v_minus_w_bound V W m + max_gain clsdiff <= level_value m w) W).
+    { move: hm.
+      generalize (v_minus_w_bound V W m) => vbound.
+      eapply LevelSetProp.fold_rec.
+      intros. intros x hin. firstorder eauto.
+      intros x a s' s'' inw nins' hadd ih heq.
+      forward ih by lia.
+      intros l hin.
+      apply hadd in hin as [].
+      * subst x. lia.
+      * now apply ih. }
+    clear hm.
+    eapply ClausesFact.for_all_iff. tc.
+    intros cl hl.
+    unfold valid_clause.
+    case: Z.ltb_spec => // hk0.
+    destruct cl as [prem [l k]] => /=.
+    eapply Nat.leb_le. cbn in hk0.
+    specialize (clw l).
+    rewrite /clsdiff in hl. eapply Clauses.diff_spec in hl as [hl hl'].
+    eapply in_clauses_with_concl in hl as [lW incls].
+    specialize (H _ lW). cbn -[clsdiff] in H. cbn in lW.
+    etransitivity; tea.
+    set (prem' := non_W_atoms W prem).
+    assert (ne : LevelExprSet.is_empty prem' = false). todo "invariant".
+    set (preml := {| t_set := prem'; t_ne := ne |}).
+
+    assert (Z.to_nat (min_premise m prem) <= 
+      Z.to_nat (min_premise_value m preml) - premise_min prem).
+    { unfold min_premise. unfold premise_min. todo "monotone". }
+    transitivity (k + (Z.to_nat (min_premise_value m preml) - premise_min prem)). lia.
+    assert (Z.to_nat (gain (prem, (l, k))) <= max_gain clsdiff). todo "easy".
+    transitivity (v_minus_w_bound V W m + Z.to_nat (gain (prem, (l, k)))).
+    2:lia.
+    unfold gain. cbn -[min_premise_value].
+    assert (premise_min prem <= (Z.to_nat (min_premise_value m preml))).
+    { todo "unclear". }
+    assert (k + (Z.to_nat (min_premise_value m preml) - premise_min prem) =
+      (Z.to_nat (min_premise_value m preml) + k - premise_min prem)) as ->. lia.
+    rewrite Z2Nat.inj_sub. lia.
+    rewrite !Nat2Z.id.
+    assert (Z.to_nat (min_premise_value m preml) <= v_minus_w_bound V W m).
+    { todo "clearly a subset". }
+    lia.
+  Qed.
+
+  Lemma is_model_equal {cls cls' m} : Clauses.Equal cls cls' -> is_model cls m -> is_model cls' m.
+  Proof. now intros ->. Qed.
+
+  Lemma union_diff_eq {cls cls'} : Clauses.Equal (Clauses.union cls (Clauses.diff cls' cls)) 
+    (Clauses.union cls cls').
+  Proof. clsets. Qed.
+
+  Lemma valid_clause_le {cl m m'} : m ⩽ m' -> valid_clause m cl -> valid_clause m' cl.
+  Proof.
+    intros hle.
+    unfold valid_clause.
+    case: Z.ltb_spec => //.
+    case: Z.ltb_spec => //.
+    - intros premge premlt.
+      intros _.
+      destruct cl as [prem [l k]]. cbn in *.
+  Abort.
+    
+  Lemma is_model_closed {cls m m'} : m ⩽ m' -> is_model cls m -> is_model cls m'.
+  Proof.
+    intros lem.
+    unfold is_model.
+    rewrite /is_true -!ClausesFact.for_all_iff.
+    intros ha x hin. specialize (ha x hin).
+    cbn in ha.
+  Abort.
 
   #[tactic="idtac"]
-  Equations? inner_loop (W : LevelSet.t) (cls : clauses) (m : model) 
-    (prf : strict_subset W V /\ ~ LevelSet.Empty W) : result W 
-    by wf (measure W cls m) lt :=
-    inner_loop W cls m subWV with inspect (measure W cls m) := {
-    | exist 0 eq => Model W m _
-    | exist (S n) neq with loop W (cls ⇂ W) m _ _ := {
+  Equations? inner_loop (W : LevelSet.t) (cls : clauses) (init : model) 
+    (m : valid_model W init (cls ⇂ W))
+    (prf : [/\ strict_subset W V, ~ LevelSet.Empty W & clauses_conclusions cls ⊂_lset W]) : 
+    result W (cls ↓ W) m.(model_model)
+    by wf (measure W cls m.(model_model)) lt :=
+    inner_loop W cls init m subWV with inspect (measure W cls m.(model_model)) := {
+    | exist 0 eq => Model W {| model_model := m.(model_model) |} _
+    | exist (S n) neq with loop W (cls ⇂ W) m.(model_model) _ _ := {
       | Loop => Loop
       (* We check if the model [mr] for (cls ⇂ W) extends to a model of (cls ↓ W). *)
-      | Model Wr mr hsub with inspect (check_model (Clauses.diff (cls ↓ W) (cls ⇂ W)) (Wr, m)) := { 
-        | exist None eqm => Model W m _
+      | Model Wr mr hsub with inspect (check_model (Clauses.diff (cls ↓ W) (cls ⇂ W)) (Wr, mr.(model_model))) := { 
+        | exist None eqm => Model W {| model_model := mr.(model_model) |} _
         | exist (Some (Wconcl, mconcl)) eqm := 
           (* If it doesn't extend, then we're entitled to recursively compute a 
               better model starting with mconcl, as we have made the measure decrease:
-              some atom that is necessarily not in W has been updated. *)
-          inner_loop W (Clauses.diff (cls ↓ W) (cls ⇂ W)) mconcl _ } } }.
-    
+              some atom in Wr has been strictly updated in Wconcl. *)
+          extends_model _ _ _ (inner_loop W cls init (* (Clauses.diff (cls ↓ W) (cls ⇂ W))  *) {| model_model := mconcl |} _) } } }.
   Proof.
-    all:clear loop inner_loop.
-    - eapply LevelSet.subset_spec; reflexivity.
+    all:cbn [model_model]; clear loop inner_loop.
+    all:try solve [try apply LevelSet.subset_spec; try reflexivity].
+    all:try apply LevelSet.subset_spec in hsub.
+    all:destruct subWV as [WV neW clsW].
+    all:try solve [intuition auto].
+    - apply clauses_conclusions_clauses_with_concl.
+    - rewrite check_model_is_model.
+      eapply is_model_equal. 2:eapply is_model_union.
+      2:{ pose proof (model_ok m). eapply check_model_is_model in H. exact H. }
+      2:{ eapply measure_model. exact clsW. exact eq. }
+      rewrite union_diff_eq.
+      enough (cls ⇂ W ⊂_clset (cls ↓ W)) by clsets.
+      { intros cl.
+        move/in_restrict_clauses => [hin hcl].
+        now rewrite in_clauses_with_concl. }
     - apply clauses_conclusions_restrict_clauses.
     - now eapply strict_subset_cardinal.
-    - auto. 
+    - apply check_model_update in eqm as []. cbn in H0.
+       transitivity (model_model mr) => //. apply mr.
+    - intuition auto.
+      eapply check_model_spec in eqm as [wrsub subwr hm dom out].
+      transitivity mr.(model_model) => //. apply mr.
+    - eapply check_model_spec in eqm as [wrsub subwr hm dom out].
+      transitivity mr.(model_model) => //. apply mr.
+      eapply model_map_outside_weaken; tea.
+      etransitivity; tea.
+      intros x.
+      rewrite LevelSet.union_spec; move => []; try lsets.
+      now move/clauses_conclusions_diff_left.
+    - eapply clauses_conclusions_restrict_clauses.
+    - rewrite check_model_is_model.
+      have okm := model_ok mr.
+      rewrite check_model_is_model in okm.
+      pose proof (check_model_update eqm) as [nmodel lem]. cbn in lem.
+      
+    
     - unfold measure.
       destruct subWV as [subWV ne].
-      eapply check_model_spec in eqm as [wrsub [subwr hm]].
+      pose proof (check_model_update eqm) as [nmodel lem].
+      eapply check_model_spec in eqm as [wrsub subwr hm hout].
       destruct hm as [l [hinw hl]].
-      rewrite !LevelSet.fold_spec.
-      eapply fold_left_ne_lt. todo "easy".
-      intros.
       assert (v_minus_w_bound V W mconcl = v_minus_w_bound V W m) as ->. 
-      { (* todo: because we don't touch V - W levels *)
-        todo "vbound".
-      }
-      assert (max_gain (Clauses.diff (clauses_with_concl cls W) (restrict_clauses cls W)) <=
-        max_gain cls).
-      { todo " as the restricted clauses are a subset of W ". }
-      assert (level_value mconcl x >= level_value m x).
-      { todo " as the improvements to the model are monotonous". }
-      lia.
-      exists l. split.
-      { epose proof (clauses_conclusions_diff_left cls W (restrict_clauses cls W)).
-        eapply LevelSet_In_elements.
-        eapply LevelSet.subset_spec in hsub.
-        lsets. }
-      intros acc.
-      assert (v_minus_w_bound V W mconcl = v_minus_w_bound V W m) as ->.
-      { todo " vbound ". }
-      assert (max_gain (Clauses.diff (clauses_with_concl cls W) (restrict_clauses cls W)) <=
-        max_gain cls).
-      { todo "same". }
-      assert (level_value mconcl l <=
-        v_minus_w_bound V W m + max_gain (Clauses.diff (clauses_with_concl cls W) (restrict_clauses cls W))).
-      { todo "the new value for l is bounded ". }
+      { (* Because we don't touch V - W levels *)
+        cbn in lem. pose proof (model_above mr).
+        symmetry.
+        apply v_minus_w_bound_irrel.
+        transitivity mr.(model_model). apply mr.
+        eapply model_map_outside_weaken; tea.
+        etransitivity; tea.
+        intros l'.
+        rewrite LevelSet.union_spec; move => []; try lsets.
+        now move/clauses_conclusions_diff_left. }
+      assert (hmaxgain : max_gain (Clauses.diff (cls ↓ W) (cls ⇂ W)) <= max_gain cls).
+      { apply max_gain_subset. intros cl. rewrite Clauses.diff_spec; move=> [].
+        now move/in_clauses_with_concl. }
+      rewrite !LevelSet.fold_spec.
+      eapply fold_left_ne_lt.
+      { destruct ne. intros he. apply H0. now rewrite LevelSetProp.elements_Empty. }
+      + intros.
+        assert (level_value m x <= level_value mconcl x).
+        { cbn in lem. have mmr := (model_above mr). 
+          eapply model_le_values. now transitivity mr.(model_model). }
         lia.
-    - eapply LevelSet.subset_spec. reflexivity.
+      + exists l. split.
+        { epose proof (clauses_conclusions_diff_left cls W (restrict_clauses cls W)).
+          eapply LevelSet_In_elements. lsets. }
+        intros acc acc' hacc.
+        assert (level_value mconcl l <= v_minus_w_bound V W m + max_gain cls).
+        { destruct hl. lia. }
+        assert (level_value m l <= level_value (model_model mr) l).
+        { eapply model_le_values. apply mr. }
+        destruct hl. lia.
+    - apply check_model_is_model. apply check_model_is_model in eqm. 
+      pose proof (ism' := model_ok mr). apply check_model_is_model in ism'.
+      have mu := is_model_union eqm ism'.
+      rewrite /is_true -mu. apply is_model_proper => //.
+      intros x.
+      rewrite Clauses.union_spec Clauses.diff_spec.
+      intuition auto.
+      * assert (Clauses.In x (cls ↓ W)). eapply in_clauses_with_concl. split => //. apply H2.
+        eapply clauses_conclusions_spec. exists x; split => //. clsets.
+      * now eapply in_clauses_with_concl in H0 as [].
+      * now eapply in_restrict_clauses in H3 as [].
+    - apply mr.
+    - apply mr.
+    - apply mr.
   Qed.
 End InnerLoop.
 
@@ -686,7 +1240,7 @@ Equations? loop (V : LevelSet.t) (cls : clauses) (m : model) (prf : clauses_conc
     result V
   by wf (LevelSet.cardinal V) lt :=
   loop V cls m prf with inspect (check_model cls (LevelSet.empty, m)) :=
-    | exist None eqm => Model LevelSet.empty m _
+    | exist None eqm => Model LevelSet.empty {| model_clauses := cls; model_model := m |} _
     | exist (Some (W, m')) eqm with inspect (LevelSet.equal W V) := {
       | exist true eq := Loop
       (* Loop on cls|W, with |W| < |V| *)
@@ -694,14 +1248,14 @@ Equations? loop (V : LevelSet.t) (cls : clauses) (m : model) (prf : clauses_conc
         | Loop := Loop
         | Model Wr mwr hsub
           (* We have a model for (cls ⇂ W), we try to extend it to a model of (csl ↓ W). *)
-          with inner_loop V loop W (cls ↓ W) mwr _ := 
+          with inner_loop V loop W (cls ↓ W) mwr.(model_model) _ := 
           { | Loop := Loop
             | Model Wc mwc hsub'
             (* We get a model for (cls ↓ W), we check if it extends to all clauses.
                By invariant |Wc| cannot be larger than |W|.
             *)
-            with inspect (check_model cls (Wc, mwc)) :=
-            { | exist None eqm' => Model Wc mwc _
+            with inspect (check_model cls (Wc, mwc.(model_model))) :=
+            { | exist None eqm' => Model Wc {| model_clauses := cls; model_model := mwc.(model_model) |} _
               | exist (Some (Wcls, mcls)) eqm' with inspect (LevelSet.equal Wcls V) := {
                 | exist true _ := Loop
                 | exist false neq' := 
@@ -727,6 +1281,7 @@ Proof.
     split => //. lsets. 
   - eapply check_model_spec in eqm as [? []].
     destruct H2 as [l [hin _]]. specialize (H l) => //.
+  - apply clauses_conclusions_clauses_with_concl.
   - eapply clauses_conclusions_diff in H.
     rewrite LevelSet.diff_spec. intuition lsets.
   - eapply check_model_subset_clauses in eqm as []; tea.
@@ -783,14 +1338,15 @@ Lemma in_add_predecessors (V : LevelSet.t) cls :
     Clauses.In cl cls \/ LevelSet.In (LevelExpr.get_level (concl cl)) V.
 Admitted.
     
-Equations? infer (V : LevelSet.t) (cls : clauses) (prf : LevelSet.Subset (clauses_conclusions cls) V) : result V  := 
-  infer V cls prf := loop V (add_predecessors V cls) (init_model cls) _.
-Proof.
+Equations infer (V : LevelSet.t) (cls : clauses) (prf : LevelSet.Subset (clauses_conclusions cls) V) : result V  := 
+  infer V cls prf := loop V cls (init_model cls) prf.
+
+  (* Proof.
   eapply clauses_conclusions_spec in H as [cl []].
   eapply in_add_predecessors in H as [].
   eapply prf. rewrite clauses_conclusions_spec. now exists cl.
   now rewrite H0 in H.
-Qed.
+Qed. *)
 
 Definition clauses_levels (cls : clauses) : LevelSet.t := 
   Clauses.fold (fun '(cl, concl) acc => 
@@ -860,15 +1416,15 @@ Definition valuation_of_model (m : model) : LevelMap.t nat :=
 Definition print_result {V} (m : result V) :=
   match m with
   | Loop => "looping"
-  | Model w m _ => "satisfiable with model: " ^ print_level_nat_map m ^ nl ^ " W = " ^
+  | Model w m _ => "satisfiable with model: " ^ print_level_nat_map m.(model_model) ^ nl ^ " W = " ^
     print_wset w 
-    ^ nl ^ "valuation: " ^ print_level_nat_map (valuation_of_model m)
+    ^ nl ^ "valuation: " ^ print_level_nat_map (valuation_of_model m.(model_model))
   end.
   
 Definition valuation_of_result {V} (m : result V) :=
   match m with
   | Loop => "looping"
-  | Model w m _ => print_level_nat_map (valuation_of_model m)
+  | Model w m _ => print_level_nat_map (valuation_of_model m.(model_model))
   end.
 
 Eval compute in print_result test.
@@ -1094,17 +1650,10 @@ Definition print_model_premises_hold cls (m : model) :=
   if premises_hold cls m then "all premises hold"
   else "some premise doesn't hold".
 
-Definition print_premises_hold {V} (cls : clauses) (r : result V) :=
+Definition print_premises_hold {V} (r : result V) :=
   match r with
   | Loop => "looping"
-  | Model w m _ => print_model_premises_hold cls m
-  end.
-
-Ltac get_result c :=
-  let c' := eval vm_compute in c in 
-  match c' with
-  | Loop => fail "looping"
-  | Model ?w ?m _ => exact m
+  | Model w m _ => print_model_premises_hold m.(model_clauses) m.(model_model)
   end.
 
 (* Is clause [c] non-vacuous and satisfied by the model? *)
@@ -1122,18 +1671,33 @@ Definition check_cstrs (m : model) (c : ConstraintSet.t) :=
   let cls := clauses_of_constraints c in
   check_clauses m cls.
   
-Equations? infer_extension (V : LevelSet.t) (cls : clauses) (m : model) (prf : LevelSet.Subset (clauses_conclusions cls) V) : result V := 
-  | V, cls, m, prf := loop V (add_predecessors V cls) m _.
+Equations? infer_extension (V : LevelSet.t) (m : valid_model V) (cls : clauses) 
+  (prf : LevelSet.Subset (clauses_conclusions cls) V) : result V := 
+  | V, m, cls', prf := loop V (Clauses.union m.(model_clauses) cls') m.(model_model) _.
 Proof.
   eapply clauses_conclusions_spec in H as [cl []].
-  eapply in_add_predecessors in H as [].
-  eapply prf. rewrite clauses_conclusions_spec. now exists cl.
-  now rewrite H0 in H.
+  eapply Clauses.union_spec in H as [].
+  apply m.(model_clauses_conclusions). 
+  rewrite clauses_conclusions_spec. now exists cl.
+  eapply prf. rewrite clauses_conclusions_spec.
+  now exists cl. 
 Qed.
 
-Equations? infer_model_extension (V : LevelSet.t) (cls : clauses) (m : model) : result (LevelSet.union (clauses_levels cls) V) :=
-  infer_model_extension V cls m := 
-    infer_extension (LevelSet.union (clauses_levels cls) V) cls (min_model m cls) _.
+(* We weaken a valid model for V to a model for [W ∪ clauses_levels cls] by 
+   setting a minimal value for the new atoms in [clauses_levels cls \ W]
+   such that the new clauses [cls] do not hold vacuously.
+*)
+Equations? weaken_model {V : LevelSet.t} (m : valid_model V) (cls : clauses) : valid_model (LevelSet.union (clauses_levels cls) V) :=
+  weaken_model m cls := 
+    {| model_clauses := m.(model_clauses); 
+       model_model := min_model m.(model_model) cls |}.
+Proof.
+  rewrite LevelSet.union_spec. right. now apply m.
+Qed.
+
+Equations? infer_model_extension {V : LevelSet.t} (m : valid_model V) (cls : clauses) : result (LevelSet.union (clauses_levels cls) V) :=
+  infer_model_extension m cls := 
+    infer_extension (LevelSet.union (clauses_levels cls) V) (weaken_model m cls) cls _.
 Proof.
   eapply LevelSet.union_spec. left.
   now eapply in_conclusions_levels.
@@ -1148,22 +1712,22 @@ Variant enforce_result :=
 
 Definition testp := Eval vm_compute in {| model_values := (LevelMap.empty _) |}.
 
-Definition enforce_clauses cls (m : model) : option model :=
-  match infer_model_extension (model_variables m) cls m with
+Definition enforce_clauses {V} (m : valid_model V) cls : option model :=
+  match infer_model_extension m cls with
   | Loop => None
-  | Model w m _ => Some m
+  | Model w m _ => Some m.(model_model)
   end.
 
-Definition enforce_clause cl (m : model) : option model :=
-  enforce_clauses (Clauses.singleton cl) m.
+Definition enforce_clause {V} (m : valid_model V) cl : option model :=
+  enforce_clauses m (Clauses.singleton cl).
 
-Definition enforce_cstr (m : model) (c : UnivConstraint.t) :=
+Definition enforce_cstr {V} (m : valid_model V) (c : UnivConstraint.t) :=
   let cls := clauses_of_constraint c in
-  enforce_clauses cls m.
+  enforce_clauses m cls.
 
-Definition enforce_cstrs (m : model) (c : ConstraintSet.t) :=
+Definition enforce_cstrs {V} (m : valid_model V) (c : ConstraintSet.t) :=
   let cls := clauses_of_constraints c in
-  enforce_clauses cls m.
+  enforce_clauses m cls.
 
 Definition initial_cstrs :=
   (add_cstr (sup levela levelb) Eq (levelc + 1)
@@ -1196,18 +1760,28 @@ Eval vm_compute in print_result test''.
 Eval vm_compute in print_result testabeqS.
 
 Eval vm_compute in print_model_premises_hold initial_cls (init_model initial_cls).
+
+Ltac get_result c :=
+  let c' := eval vm_compute in c in 
+  match c' with
+  | Loop => fail "looping"
+  | Model ?w ?m _ => exact m
+  end.
+
 Definition model_cstrs' := ltac:(get_result test'').
 
-Eval vm_compute in check_cstrs model_cstrs' initial_cstrs.
+Eval vm_compute in check_cstrs model_cstrs'.(model_model) initial_cstrs.
 (* Here c <= b, in the model b = 0 is minimal, and b's valuation gives 1 *)
 Eval vm_compute in print_result (infer_model initial_cls).
 
-(* Here this is no longer the case! We started with b = 0 but move it to 10 
-  due to the b + 10 -> e clause, without reconsidering the b -> c clause *)
-Eval vm_compute in option_map valuation_of_model
+(* Here it is still the case, we started with b = 0 but move it to 10 
+  due to the b + 10 -> e clause, and reconsider the b -> c clause to move 
+  c up *)
+Eval vm_compute in 
+  option_map valuation_of_model
   (enforce_cstrs model_cstrs' enforced_cstrs).
 
-(* However the whole set of constraints has a finite model with c <= b *)
+(* The whole set of constraints has a finite model with c <= b *)
 
 Definition all_clauses := Clauses.union initial_cls enforced_cls.
 
@@ -1219,14 +1793,15 @@ Eval vm_compute in
 Eval vm_compute in (enforce_cstrs model_cstrs' enforced_cstrs).
 Eval vm_compute in print_clauses initial_cls.
 
-(** This is not a model of the closure of the initial clauses *)
-Eval vm_compute in
-  option_map (is_model initial_cls) 
-    (enforce_cstrs model_cstrs' enforced_cstrs).
+Notation "x ≡ y" := (eq_refl : x = y) (at level 70).
 
-(* While it is a model of the new constraints *)    
-Eval vm_compute in
-  option_map (is_model enforced_cls) (enforce_cstrs model_cstrs' enforced_cstrs).
+(** This is also a model of (the closure of) the initial clauses *)
+Check (option_map (is_model initial_cls) (enforce_cstrs model_cstrs' enforced_cstrs)
+  ≡ Some true).
+
+(* And a model of the new constraints *)
+Check (option_map (is_model enforced_cls) (enforce_cstrs model_cstrs' enforced_cstrs)
+   ≡ Some true).
 
 (* All premises hold *)    
 Eval vm_compute in 
